vale/code/crypto/ecc/curve25519/FastHybrid_helpers.fsti
@@ -70,36 +70,20 @@ val lemma_addition (a d:nat) (a0 a1 a2 a3 d0 d1 d2 d3 d4:nat64)
             c4 == 0))
   (ensures a + d == pow2_five s0 s1 s2 s3 s4)
 
-//#reset-options "--z3rlimit 20"
-let lemma_carry_wide (a0 a1 a2 a3 a4 a5 a6 a7
+val lemma_carry_wide (a0 a1 a2 a3 a4 a5 a6 a7
                       d0 d1 d2 d3 carry
                       d0' d1' d2' d3':nat64) : Lemma
   (requires pow2_five d0 d1 d2 d3 carry == 38 * pow2_four a4 a5 a6 a7 + pow2_four a0 a1 a2 a3 /\
             pow2_four d0' d1' d2' d3' % prime == ((pow2_four d0 d1 d2 d3) + carry * pow2_256) % prime)
   (ensures (pow2_four d0' d1' d2' d3') % prime == (pow2_eight a0 a1 a2 a3 a4 a5 a6 a7) % prime)
-  =
-  calc (==) {
-    pow2_four d0' d1' d2' d3' % prime;
-    == { calc (==) {
-           (pow2_four d0 d1 d2 d3) + carry * pow2_256;
-           == { _ by (int_canon()) }
-           pow2_five d0 d1 d2 d3 carry;
-         }
-       }
-    pow2_five d0 d1 d2 d3 carry % prime;
-    == {}
-    (pow2_four a0 a1 a2 a3 + 38 * pow2_four a4 a5 a6 a7) % prime;
-    == { lemma_mul_pow256_add (pow2_four a0 a1 a2 a3) (pow2_four a4 a5 a6 a7) }
-    (pow2_four a0 a1 a2 a3 + pow2_256 * pow2_four a4 a5 a6 a7) % prime;
-    == { _ by (int_canon()) }
-    (pow2_eight a0 a1 a2 a3 a4 a5 a6 a7) % prime;
-  }
-
-
-
 
 val lemma_carry_sub_prime (a0 a1 a2 a3 a0' a1' a2' a3' carry_in:nat64) (carry:bit) : Lemma
   (requires pow2_four a0' a1' a2' a3' - carry * pow2_256 == pow2_four a0 a1 a2 a3 - carry_in * 38 /\
             carry_in * 38 - 1 + 38 < pow2_64)
   (ensures a0' - carry * 38 >= 0 /\
            (pow2_four (a0' - carry * 38) a1' a2' a3') % prime == (pow2_four a0 a1 a2 a3 - carry_in * pow2_256) % prime)
+
+val lemma_fmul (a0 a1 a2 a3 b d0 d1 d2 d3 carry:nat64) : Lemma
+  (requires pow2_five d0 d1 d2 d3 carry == (pow2_four a0 a1 a2 a3) * b /\
+            b <= 121665)
+  (ensures carry * 38 < pow2_63)
